proof/correctness1024/MLKEM_Poly.ec
@@ -1683,11 +1683,11 @@ lemma poly_basemul_corr _ap _bp:
    hoare[Jkem1024.M(Jkem1024.Syscall)._poly_basemul :
      _ap = lift_array256 ap /\ _bp = lift_array256 bp /\
      signed_bound_cxq ap 0 256 2 /\  signed_bound_cxq bp 0 256 2 ==>
-     signed_bound_cxq res 0 256 3 /\ 
+     signed_bound_cxq res 0 256 2 /\ 
      lift_array256 res = scale (basemul _ap _bp) (incoeff 169)].
 proof.
 conseq (_: _ ==> 
-   signed_bound_cxq res 0 256 3 /\ 
+   signed_bound_cxq res 0 256 2 /\ 
    isbasemul _ap _bp zetas (lift_array256 res) 256).
 + move => ?? result [#] ? H; split; 1:smt().  
   by apply (basemul_sem _ap _bp  (lift_array256 result)).
@@ -1695,7 +1695,7 @@ proc.
 seq 2 : #pre; first by auto => />.
 while (#pre /\ srp = rp /\
     0<= to_uint i <= 256 /\ to_uint i %% 4 = 0 /\
-    signed_bound_cxq rp 0 (to_uint i) 3 /\
+    signed_bound_cxq rp 0 (to_uint i) 2 /\
     isbasemul _ap _bp zetas (lift_array256 rp) (to_uint i)); 
        last by auto => /> &hr ??; split; [ smt() | move => ??;rewrite ultE /#].
 
@@ -1878,7 +1878,7 @@ lemma poly_basemul_correct _ap _bp:
    phoare[Jkem1024.M(Jkem1024.Syscall)._poly_basemul :
      _ap = lift_array256 ap /\ _bp = lift_array256 bp /\
      signed_bound_cxq ap 0 256 2 /\  signed_bound_cxq bp 0 256 2 ==>
-     signed_bound_cxq res 0 256 3 /\ 
+     signed_bound_cxq res 0 256 2 /\ 
      lift_array256 res = scale (basemul _ap _bp) (incoeff 169)] =1%r 
   by conseq poly_basemul_ll (poly_basemul_corr _ap _bp). 
 
